Reorganize code in several modules

Data/Lib.hs
@@ -2,10 +2,19 @@ module Data.Lib where
 
 import qualified Prelude
 import qualified Data.List
+import qualified Data.Peano as Peano
+
+
+__ :: any
+__ = Prelude.error "Logical or arity value used"
 
 undefined :: a1
 undefined =
   Prelude.error "AXIOM TO BE REALIZED"
+
+uncurry_sig :: (a1 -> () -> a2) -> a1 -> a2
+uncurry_sig f p =
+  f p __
 
 fromMaybe :: a1 -> (Prelude.Maybe a1) -> a1
 fromMaybe d mx =
@@ -25,6 +34,10 @@ list_membership l =
    [] -> [];
    (:) x xs -> (:) x
     ((Prelude.map) (exist_in_cons x xs) (list_membership xs))}
+
+lt_sub :: Prelude.Int -> Prelude.Int -> Prelude.Int
+lt_sub n m =
+  Peano.minus m n
 
 safe_hd :: ([] a1) -> a1
 safe_hd xs =
