Compare.v
@@ -1,3 +1,5 @@
+Require Import Coq.Logic.ProofIrrelevance.
+
 (** ** Comparisons *)
 
 (** These definitions avoid boilerplate involved with setting up properly
@@ -44,3 +46,13 @@ Class CompareSpec (a : Set) := {
   cmp_eq_dec x y : { x = y } + { x <> y } :=
     mk_cmp_eq_dec x y cmp (cmp_eq_iff x y)
 }.
+
+Ltac cmp_reflexive :=
+  match goal with
+    [ |- context [match cmp_eq_dec ?X ?X with _ => _ end] ] =>
+      assert (cmp_eq_dec X X = left eq_refl) as Hrcmp
+        by (intros; destruct (cmp_eq_dec X X);
+              [ f_equal; apply proof_irrelevance
+              | intuition ]);
+      rewrite Hrcmp in *; clear Hrcmp; simpl in *
+  end.
